# 1

$$\frac{dx}{dt}=f(x)=-\nabla U(x)$$

$$dx=f(x)dt+g(x)dW(t)$$

$$\frac{dx}{dt}=f(x)=-\nabla U(x)+J(x)$$

$$U_q(x)\propto -\ln(P_s(x))$$

$$\int_0^tg(x_t)dW(t)=\lim_{n\rightarrow\infty}\sum_{k=1}^n g(x_{t_k^\star})(W(t_k)-W(t_{k-1}))$$

$$t_k^\star=t_{k-1}+\alpha(t_k-t_{k-1})$$

$$\begin{align*}
dx&=f(x)dt+g(x^\star)dW_t\\
&=f(x)dt+(g+dg)dW_t\\
&=f(x)dt+g(x)dW_t+\alpha\frac{\partial g}{\partial x}dxdW_t\\
&=f(x)dt+g(x)dW_t+\alpha\frac{\partial g}{\partial x}(f(x)dt+g(x)dW_t)dW_t\\
&=(f(x)+\alpha g(x)\frac{\partial g}{\partial x})dt+g(x)dW_t
\end{align*}$$

$$\frac{\partial}{\partial t}f(\vec{x},t)=-\sum\frac{\partial}{\partial x_i}(a_i(\vec{x})f(\vec{x},t))+\sum_i\sum_j\frac{\partial^2}{\partial x_i \partial x_j}(b_{ij}(\vec{x})f(\vec{x},t))$$

$$\frac{\partial P}{\partial t}=-\frac{\partial}{\partial x}((f+\alpha gg')P)+\frac{1}{2}\frac{\partial^2}{\partial x^2}(g^2P)=0$$

$$\begin{align*}
\frac{\partial}{\partial x}((f+\alpha gg')P)=&\frac{1}{2}\frac{\partial^2}{\partial x^2}(g^2P)\\
(f+\alpha gg')P=&\frac{1}{2}\frac{\partial}{\partial x}(g^2P)\\
(f+\alpha gg')(g^2P)=&\frac{g^2}{2}\frac{\partial}{\partial x}(g^2P)
\end{align*}$$

$$P_s(x)=\frac{N}{g^2(x)}\exp(2\int^x\frac{f(z)+\alpha g(z)g'(z)}{g^2(z)}dz)$$

$$U(x)=\frac{x^4}{4}-\frac{x^2}{2}$$

$$g(x)=\sigma$$

$$P_s(x)=\frac{N}{\sigma^2}\exp(\frac{-2U(x)}{\sigma^2})$$

$$U_q(x)=\frac{2U_(x)}{\sigma^2}+\ln(\frac{\sigma^2}{N})$$

$$g(x)=\frac{\sigma}{4}(x^4-4x^2+8)$$

$$P_s(x)=\frac{16N}{\sigma^2}\exp ( 2(\alpha-1)\ln(x^4-4x^2+8)\\
+\frac{1}{\sigma^2}(\tan^{-1}(1-\frac{x^2}{2}-\frac{2(x^2-6)}{x^2-4x+8})+C)$$

$$U_q(x)=\ln(\frac{\sigma^2}{16N}(x^4-4x^2+8)^{2(1-\alpha)})\\
-\frac{1}{\sigma^2}(\tan^{-1}(1-\frac{x^2}{2})-\frac{2(x^2-6)}{x^4-4x^2+8})$$

$$g(x)=\sigma(1+x^2)$$

$$P_s(x)=\frac{N}{\sigma^2(1+x^2)^2}\exp(\frac{1}{\sigma^2}(2\alpha\sigma^2-1)\ln(1+x^2)-\frac{2}{1+x^2}+C)$$

$$U_q(x)=\ln(\frac{\sigma^2(1+x^2)^2}{N})-\frac{1}{\sigma^2}((2\alpha\sigma^2-1)\ln(1+x^2)-\frac{2}{1+x^2}+C)$$

$$x_{min}=\pm\sqrt{\frac{1-2\sigma^2(1-\alpha)}{1+2\sigma^2(1-\alpha)}}$$

$$\sigma_{c,\alpha}=\frac{1}{\sqrt{2(1-\alpha)}}$$

$$\frac{dx}{dt}=-k_1x^3+k_2x^2-k_3x+k_4$$

$$U(x)=\frac{k_1x^4}{4}-\frac{k_2x^3}{3}+\frac{k_3x^2}{2}+k_4x$$

$$dx=(-k_1x^3+k_2x^2-k_3x+k_4)dt+\sigma\sqrt{k_1x^3+k_2x^2+k_3x+k_4}dW_t$$

$$P_s(x)=\frac{N}{k_1x^3+k_2x^2+k_3x+k_4}\exp(2\int^x\frac{-k_1z^3+k_2z^2-k_3z+k_4}{k_1z^3+k_2z^2+k_3z+k_4}dz)$$

$$A+2X\rightleftharpoons^{c_1}_{c_2} 3X$$

$$B\rightleftharpoons^{c_4}_{c_3}X$$

$$g(x)=\sigma(U(x)+C)^\delta$$

$$f(x)=\frac{1}{P_s(x)}\frac{\partial}{\partial x}(\frac{g^2P_s}{2})-\alpha g g'$$

$$(f+\alpha gg')P=\frac{1}{2}\frac{\partial}{\partial x}(g^2P)$$

$$fP_s+\alpha gg'P_s=\frac{1}{2}g^2P_s'+gg'P_s$$

$$\alpha=1,g(x)=\sqrt{\frac{2}{P_s'(x)}P_s(x)f'(x)}$$

$$\alpha \ne 1, g(x)=\sqrt{\frac{2}{1-\alpha}P_s^{1/(\alpha-1)}\int^x fP_s^{-1/(\alpha-1)}}$$

$$f_1(x)=-x$$

$$g_1(x)=\sigma\exp(-x^2)$$

$$f_2=2x-\frac{1}{4}x\exp(2x^2)$$

$$g_2=1$$