# 1

$$\frac{dH}{dt} = k_1 \frac{(1 - \alpha) S^{n_1} + K_{M1}^{n_1}}{S^{n_1} + K_{M1}^{n_1}} \frac{H^{n_2}}{H^{n_2} + K_{M2}^{n_2}} + k_2 - k_3 H$$

$$\frac{dS}{dt} = k_4 \frac{(1 - \beta) H^{n_3} + K_{M3}^{n_3}}{H^{n_3} + K_{M3}^{n_3}} \frac{S^{n_4}}{S^{n_4} + K_{M4}^{n_4}} (S_{total} - S) + k_5 - k_6 S$$

$$
\frac{dS}{dt} = \left( \beta_1 + \frac{S^{n_1}}{K_S^{n_1} + S^{n_1}} \right) (S_{total}(D) - S) - (d_S + \gamma_1 \cdot H) S
$$

$$
\frac{dH}{dt} = \left( \beta_2 + \frac{H^{n_2}}{K_H^{n_2} + H^{n_2}} \right) (H_{total}(D) - H) - (d_H + \gamma_2 \cdot S) H
$$

$$
S_{total}(D) = a_{St} \frac{K_{St}^3}{K_{St}^3 + D^3} + k_{St} D + b_{St}
$$

$$
H_{total}(D) = a_{Ht} \frac{K_{Ht}^3}{K_{Ht}^3 + D^3} + k_{Ht} D + b_{Ht}
$$